13MachineCode/Disassemble.thy
@@ -7,31 +7,29 @@ primrec register_map :: "register \<Rightarrow> reg" where
 | "register_map Env = R2"
 | "register_map Vals = R3"
 | "register_map Stk = R4"
+| "register_map Acc = R5"
 
 primrec register_offset :: "register \<Rightarrow> nat" where
   "register_offset Hp = 0"
 | "register_offset Env = 1"
 | "register_offset Vals = 2"
 | "register_offset Stk = 3"
+| "register_offset Acc = 4"
 
-fun pseudoreg_size :: "move_src \<Rightarrow> nat" where
-  "pseudoreg_size (Reg (Some r)) = 4"
-| "pseudoreg_size (Reg None) = 1"
+primrec pseudoreg_size :: "move_src \<Rightarrow> nat" where
+  "pseudoreg_size (Reg r) = (if r = Acc then 1 else 4)"
 | "pseudoreg_size (Con k) = 1"
 
-fun pseudoreg_map :: "register option \<times> nat \<Rightarrow> nat" where
-  "pseudoreg_map (Some r, x) = 4 * x + register_offset r"
-| "pseudoreg_map (None, x) = x"
+primrec pseudoreg_map :: "register \<times> nat \<Rightarrow> nat" where
+  "pseudoreg_map (r, x) = (if r = Acc then x else 4 * x + register_offset r)"
 
 fun disassemble' :: "assm \<Rightarrow> mach" where
-  "disassemble' (AGet r) = LOD R5 (case r of Some r \<Rightarrow> register_map r | None \<Rightarrow> R5)"
-| "disassemble' (APut (Some r) (Reg r')) = 
-    STO (register_map r) (case r' of Some r' \<Rightarrow> register_map r' | None \<Rightarrow> R5)"
-| "disassemble' (APut (Some r) (Con k)) = STI (register_map r) k"
-| "disassemble' (APut None (Reg r)) = MOV R5 (case r of Some r \<Rightarrow> register_map r | None \<Rightarrow> R5)"
-| "disassemble' (APut None (Con k)) = LDI R5 k"
-| "disassemble' (ASub r k) = SUB (case r of Some r \<Rightarrow> register_map r | None \<Rightarrow> R5) (4 * k)"
-| "disassemble' (AAdd r k) = ADD (case r of Some r \<Rightarrow> register_map r | None \<Rightarrow> R5) (4 * k)"
+  "disassemble' (AGet r) = LOD R5 (register_map r)"
+| "disassemble' (APut r (Reg r')) = 
+    (if r = Acc then MOV R5 (register_map r') else STO (register_map r) (register_map r'))"
+| "disassemble' (APut r (Con k)) = (if r = Acc then LDI R5 k else STI (register_map r) k)"
+| "disassemble' (ASub r k) = SUB (register_map r) (4 * k)"
+| "disassemble' (AAdd r k) = ADD (register_map r) (4 * k)"
 | "disassemble' AJmp = JMP R5"
 
 definition disassemble :: "assm list \<Rightarrow> mach list" where
@@ -44,15 +42,15 @@ fun unmap_mem' :: "nat \<Rightarrow> register \<times> nat" where
 | "unmap_mem' (Suc (Suc (Suc 0))) = (Stk, 0)"
 | "unmap_mem' (Suc (Suc (Suc (Suc x)))) = (case unmap_mem' x of (a, b) \<Rightarrow> (a, Suc b))"
 
-definition unmap_mem :: "(register option \<Rightarrow> nat \<Rightarrow> register option \<times> nat) \<Rightarrow> nat \<Rightarrow> nat" where
-  "unmap_mem m x = (case unmap_mem' x of (r, p) \<Rightarrow> pseudoreg_map (m (Some r) p))"
+definition unmap_mem :: "(register \<Rightarrow> nat \<Rightarrow> register \<times> nat) \<Rightarrow> nat \<Rightarrow> nat" where
+  "unmap_mem m x = (case unmap_mem' x of (r, p) \<Rightarrow> pseudoreg_map (m r p))"
 
-primrec inv_register_map :: "(register option \<Rightarrow> nat) \<Rightarrow> register option \<Rightarrow> reg \<Rightarrow> nat" where
-  "inv_register_map rs t R1 = rs (Some Hp) * 4"
-| "inv_register_map rs t R2 = rs (Some Env) * 4 + 1"
-| "inv_register_map rs t R3 = rs (Some Vals) * 4 + 2"
-| "inv_register_map rs t R4 = rs (Some Stk) * 4 + 3"
-| "inv_register_map rs t R5 = pseudoreg_map (t, rs None)"
+primrec inv_register_map :: "(register \<Rightarrow> nat) \<Rightarrow> register \<Rightarrow> reg \<Rightarrow> nat" where
+  "inv_register_map rs t R1 = rs Hp * 4"
+| "inv_register_map rs t R2 = rs Env * 4 + 1"
+| "inv_register_map rs t R3 = rs Vals * 4 + 2"
+| "inv_register_map rs t R4 = rs Stk * 4 + 3"
+| "inv_register_map rs t R5 = pseudoreg_map (t, rs Acc)"
 
 primrec disassemble_state :: "assm_state \<Rightarrow> mach_state" where
   "disassemble_state (AS mem rs t pc) = MS (inv_register_map rs t) (unmap_mem mem) pc"
@@ -72,7 +70,7 @@ lemma [dest]: "R3 = register_map r \<Longrightarrow> r = Vals"
 lemma [dest]: "R4 = register_map r \<Longrightarrow> r = Stk"
   by (induction r) simp_all
 
-lemma [dest]: "R5 = register_map r \<Longrightarrow> False"
+lemma [dest]: "R5 = register_map r \<Longrightarrow> r = Acc"
   by (induction r) simp_all
 
 lemma unmap_times_4 [simp]: "unmap_mem' (4 * k) = (Hp, k)"
@@ -96,6 +94,9 @@ lemma [dest]: "unmap_mem' x = (Vals, ps Vals) \<Longrightarrow> x = Suc (Suc (ps
 lemma [dest]: "unmap_mem' x = (Stk, ps Stk) \<Longrightarrow> x = Suc (Suc (Suc (ps Stk * 4)))"
   by (induction x arbitrary: ps rule: unmap_mem'.induct) (auto split: prod.splits)
 
+lemma [dest]: "unmap_mem' x = (Acc, b) \<Longrightarrow> False"
+  by (induction x arbitrary: b rule: unmap_mem'.induct) (auto split: prod.splits)
+
 lemma [simp]: "unmap_mem' 2 = (Vals, 0)"
   by (simp add: numeral_def)
 
@@ -105,25 +106,30 @@ proof -
   thus ?thesis by simp
 qed
 
-lemma inv_reg_map_reg: "
+lemma inv_reg_map_reg: "r \<noteq> Acc \<Longrightarrow>
   (inv_register_map ps act)(R5 := inv_register_map ps act (register_map r)) = 
-    inv_register_map (ps(None := ps (Some r))) (Some r)"
+    inv_register_map (ps(Acc := ps r)) r"
 proof
   fix x
-  show "((inv_register_map ps act)(R5 := inv_register_map ps act (register_map r))) x = 
-      inv_register_map (ps(None := ps (Some r))) (Some r) x"
+  assume "r \<noteq> Acc"
+  thus "((inv_register_map ps act)(R5 := inv_register_map ps act (register_map r))) x = 
+      inv_register_map (ps(Acc := ps r)) r x"
   proof (induction x)
     case R5
     thus ?case by (induction r) simp_all
   qed simp_all
 qed
 
-lemma inv_reg_map_none: "(inv_register_map ps act)(R5 := k) = inv_register_map (ps(None := k)) None"
+lemma inv_reg_map_none: "(inv_register_map ps act)(R5 := k) = inv_register_map (ps(Acc := k)) Acc"
 proof
   fix x
-  show "((inv_register_map ps act)(R5 := k)) x = inv_register_map (ps(None := k)) None x"
+  show "((inv_register_map ps act)(R5 := k)) x = inv_register_map (ps(Acc := k)) Acc x"
     by (induction x) simp_all
 qed
+
+lemma [simp]: "(inv_register_map ps act)
+    (R5 := if act = Acc then ps Acc else 4 * ps Acc + register_offset act) = inv_register_map ps act"
+  by auto
 
 lemma [simp]: "unmap_mem' (k * 4) = (Hp, k)"
   by (induction k) (simp_all add: numeral_def)
@@ -137,89 +143,90 @@ lemma [simp]: "unmap_mem' (Suc (Suc (k * 4))) = (Vals, k)"
 lemma [simp]: "unmap_mem' (k * 4 + 3) = (Stk, k)"
   by (induction k) (simp_all add: numeral_def)
 
-lemma [simp]: "unmap_mem' (4 * k + register_offset m) = (m, k)"
+lemma [simp]: "m \<noteq> Acc \<Longrightarrow> unmap_mem' (4 * k + register_offset m) = (m, k)"
 proof (induction k)
   case 0
   thus ?case by (induction m) (simp_all add: numeral_def)
 qed (simp_all add: numeral_def)
 
-lemma [simp]: "inv_register_map (ps(Some r := k)) act R5 = inv_register_map ps act R5"
+lemma [simp]: "r \<noteq> Acc \<Longrightarrow> inv_register_map (ps(r := k)) act R5 = inv_register_map ps act R5"
   by (induction act) simp_all
 
-lemma [simp]: "inv_register_map (ps(Some r := ps (Some r) + k)) act = 
-  ((inv_register_map ps act)
-    (register_map r := inv_register_map ps act (register_map r) + 4 * k))"
+lemma [simp]: "r \<noteq> Acc \<Longrightarrow> inv_register_map (ps(r := ps r + k)) act = 
+  ((inv_register_map ps act) (register_map r := inv_register_map ps act (register_map r) + 4 * k))"
 proof
   fix x
-  show "inv_register_map (ps(Some r := ps (Some r) + k)) act x =
-    ((inv_register_map ps act)
+  assume "r \<noteq> Acc"
+  thus "inv_register_map (ps(r := ps r + k)) act x =
+    ((inv_register_map ps act) 
       (register_map r := inv_register_map ps act (register_map r) + 4 * k)) x" 
     by (induction x) auto
 qed
 
-lemma [simp]: "(inv_register_map ps (Some r)) (R5 := 4 * ps None + register_offset r + 4 * k) = 
-  inv_register_map (ps(None := ps None + k)) (Some r)"
+lemma [simp]: "r \<noteq> Acc \<Longrightarrow> (inv_register_map ps r) (R5 := 4 * ps Acc + register_offset r + 4 * k) = 
+  inv_register_map (ps(Acc := ps Acc + k)) r"
 proof
   fix x
-  show "((inv_register_map ps (Some r)) (R5 := 4 * ps None + register_offset r + 4 * k)) x =
-    inv_register_map (ps(None := ps None + k)) (Some r) x" by (induction x) simp_all
+  assume "r \<noteq> Acc"
+  thus "((inv_register_map ps r) (R5 := 4 * ps Acc + register_offset r + 4 * k)) x =
+    inv_register_map (ps(Acc := ps Acc + k)) r x" by (induction x) simp_all
 qed
 
-lemma [simp]: "ps (Some r) \<ge> k \<Longrightarrow>
-  inv_register_map (ps(Some r := ps (Some r) - k)) act = ((inv_register_map ps act)
+lemma [simp]: "ps r \<ge> k \<Longrightarrow> r \<noteq> Acc \<Longrightarrow>
+  inv_register_map (ps(r := ps r - k)) act = ((inv_register_map ps act)
     (register_map r := inv_register_map ps act (register_map r) - 4 * k))"
 proof
   fix x
-  assume "ps (Some r) \<ge> k"
-  thus "inv_register_map (ps(Some r := ps (Some r) - k)) act x =
+  assume "ps r \<ge> k" and "r \<noteq> Acc"
+  thus "inv_register_map (ps(r := ps r - k)) act x =
     ((inv_register_map ps act) 
       (register_map r := inv_register_map ps act (register_map r) - 4 * k)) x" 
     by (induction x) auto
 qed
 
-lemma [simp]: "ps None \<ge> k \<Longrightarrow> 
-  (inv_register_map ps (Some r)) (R5 := 4 * ps None + register_offset r - 4 * k) = 
-    inv_register_map (ps(None := ps None - k)) (Some r)"
+lemma [simp]: "ps Acc \<ge> k \<Longrightarrow> r \<noteq> Acc \<Longrightarrow>
+  (inv_register_map ps r) (R5 := 4 * ps Acc + register_offset r - 4 * k) = 
+    inv_register_map (ps(Acc := ps Acc - k)) r"
 proof
   fix x
-  assume "ps None \<ge> k"
-  thus "((inv_register_map ps (Some r))
-    (R5 := 4 * ps None + register_offset r - 4 * k)) x = 
-      inv_register_map (ps(None := ps None - k)) (Some r) x" 
+  assume "ps Acc \<ge> k" and "r \<noteq> Acc"
+  thus "((inv_register_map ps r) (R5 := 4 * ps Acc + register_offset r - 4 * k)) x = 
+      inv_register_map (ps(Acc := ps Acc - k)) r x" 
     by (induction x) simp_all
 qed
 
-lemma [simp]: "unmap_mem mem (inv_register_map ps (Some r) (register_map r)) = 
-    pseudoreg_map (mem (Some r) (ps (Some r)))"
+lemma [simp]: "r \<noteq> Acc \<Longrightarrow> unmap_mem mem (inv_register_map ps r (register_map r)) = 
+    pseudoreg_map (mem r (ps r))"
   by (induction r) (simp_all add: unmap_mem_def split: prod.splits)
 
-lemma [simp]: "mem (Some r) (ps (Some r)) = (t, b) \<Longrightarrow> 
+lemma [simp]: "r \<noteq> Acc \<Longrightarrow> mem r (ps r) = (t, b) \<Longrightarrow> 
   (inv_register_map ps act)(R5 := unmap_mem mem (inv_register_map ps act (register_map r))) = 
-    inv_register_map (ps(None := b)) t"
+    inv_register_map (ps(Acc := b)) t"
 proof
   fix x
-  assume "mem (Some r) (ps (Some r)) = (t, b)"
+  assume "mem r (ps r) = (t, b)" and "r \<noteq> Acc"
   thus "((inv_register_map ps act)(R5 := 
     unmap_mem mem (inv_register_map ps act (register_map r)))) x = 
-      inv_register_map (ps(None := b)) t x"
+      inv_register_map (ps(Acc := b)) t x"
   proof (induction x)
     case R5
     thus ?case by (induction r) (simp_all add: unmap_mem_def)
   qed simp_all
 qed
 
-lemma unmap_upd_k: "(unmap_mem mem)(inv_register_map ps act (register_map r) := k) = 
-    unmap_mem (mem_upd mem (Some r) (ps (Some r)) (None, k))"
+lemma unmap_upd_k: "r \<noteq> Acc \<Longrightarrow> (unmap_mem mem)(inv_register_map ps act (register_map r) := k) = 
+    unmap_mem (mem_upd mem r (ps r) (Acc, k))"
   by (rule, induction r) (auto simp add: unmap_mem_def split: prod.splits)
 
-lemma [simp]: "((unmap_mem mem)
+lemma [simp]: "r \<noteq> Acc \<Longrightarrow> r' \<noteq> Acc \<Longrightarrow> ((unmap_mem mem)
   (inv_register_map ps act (register_map r) := inv_register_map ps act (register_map r'))) = 
-    unmap_mem (mem_upd mem (Some r) (ps (Some r)) (Some r', ps (Some r')))"
+    unmap_mem (mem_upd mem r (ps r) (r', ps r'))"
 proof
   fix x
-  show "((unmap_mem mem)
+  assume "r \<noteq> Acc" and "r' \<noteq> Acc"
+  thus "((unmap_mem mem)
     (inv_register_map ps act (register_map r) := inv_register_map ps act (register_map r'))) x = 
-      unmap_mem (mem_upd mem (Some r) (ps (Some r)) (Some r', ps (Some r'))) x"
+      unmap_mem (mem_upd mem r (ps r) (r', ps r')) x"
   proof (induction r)
     case Hp
     thus ?case by (induction r') (auto simp add: unmap_mem_def split: prod.splits)
@@ -232,30 +239,33 @@ proof
   next
     case Stk
     thus ?case by (induction r') (auto simp add: unmap_mem_def split: prod.splits)
-  qed
+  qed simp_all
 qed
 
-lemma [simp]: "((unmap_mem mem)(inv_register_map ps act (register_map r) := 
-    pseudoreg_map (act, a))) = unmap_mem (mem_upd mem (Some r) (ps (Some r)) (act, a))"
+lemma [simp]: "r \<noteq> Acc \<Longrightarrow> ((unmap_mem mem)(inv_register_map ps act (register_map r) := 
+  (if act = Acc then a else 4 * a + register_offset act))) = 
+    unmap_mem (mem_upd mem r (ps r) (act, a))"
 proof
   fix x
-  show "((unmap_mem mem)(inv_register_map ps act (register_map r) := 
-    pseudoreg_map (act, a))) x = unmap_mem (mem_upd mem (Some r) (ps (Some r)) (act, a)) x"
-      by (induction r) (auto simp add: unmap_mem_def split: prod.splits)
+  assume "r \<noteq> Acc"
+  thus "((unmap_mem mem)(inv_register_map ps act (register_map r) := 
+    (if act = Acc then a else 4 * a + register_offset act))) x = 
+      unmap_mem (mem_upd mem r (ps r) (act, a)) x"
+        by (induction r) (auto simp add: unmap_mem_def split: prod.splits)
 qed
 
-lemma [simp]: "mem (Some m) (ps None) = (t, b) \<Longrightarrow>  
-  ((inv_register_map ps (Some m))(R5 := unmap_mem mem (4 * ps None + register_offset m))) = 
-    inv_register_map (ps(None := b)) t"
+lemma [simp]: "m \<noteq> Acc \<Longrightarrow> mem m (ps Acc) = (t, b) \<Longrightarrow>  
+  ((inv_register_map ps m)(R5 := unmap_mem mem (4 * ps Acc + register_offset m))) = 
+    inv_register_map (ps(Acc := b)) t"
 proof 
   fix x
-  assume "mem (Some m) (ps None) = (t, b)"
-  thus "((inv_register_map ps (Some m))(R5 := unmap_mem mem (4 * ps None + register_offset m))) 
-    x = inv_register_map (ps(None := b)) t x"
+  assume "mem m (ps Acc) = (t, b)" and "m \<noteq> Acc"
+  thus "((inv_register_map ps m)(R5 := unmap_mem mem (4 * ps Acc + register_offset m))) 
+    x = inv_register_map (ps(Acc := b)) t x"
       by (induction x) (auto simp add: unmap_mem_def)
 qed
 
-lemma [simp]: "(inv_register_map ps act)(R5 := pseudoreg_map (act, ps None)) = inv_register_map ps act"
+lemma [simp]: "(inv_register_map ps act)(R5 := pseudoreg_map (act, ps Acc)) = inv_register_map ps act"
   by auto
 
 lemma lookup_disassemble [simp]: "lookup cd pc = Some op \<Longrightarrow> disassemble cd ! pc = disassemble' op"
@@ -268,15 +278,19 @@ theorem correctm [simp]: "cd\<^sub>a \<tturnstile> \<Sigma>\<^sub>a \<leadsto>\<
   disassemble cd\<^sub>a \<tturnstile> disassemble_state \<Sigma>\<^sub>a \<leadsto>\<^sub>m disassemble_state \<Sigma>\<^sub>a'"
 proof (induction cd\<^sub>a \<Sigma>\<^sub>a \<Sigma>\<^sub>a' rule: evala.induct)
   case (eva_movr cd pc r mem ps act)
-  hence "disassemble cd \<tturnstile> MS (inv_register_map ps act) (unmap_mem mem) (Suc pc) \<leadsto>\<^sub>m 
+  moreover hence "disassemble cd \<tturnstile> MS (inv_register_map ps act) (unmap_mem mem) (Suc pc) \<leadsto>\<^sub>m 
     MS ((inv_register_map ps act)(R5 := (inv_register_map ps act) (register_map r))) 
       (unmap_mem mem) pc" by simp
-  thus ?case by (simp add: inv_reg_map_reg)
+  ultimately show ?case by (simp add: inv_reg_map_reg)
 next
   case (eva_mova cd pc mem ps act)
+  hence "disassemble cd ! pc = MOV R5 R5" by simp
   hence "disassemble cd \<tturnstile> MS (inv_register_map ps act) (unmap_mem mem) (Suc pc) \<leadsto>\<^sub>m 
-    MS ((inv_register_map ps act)(R5 := (inv_register_map ps act) R5)) 
-      (unmap_mem mem) pc" by simp
+    MS ((inv_register_map ps act)(R5 := inv_register_map ps act R5)) (unmap_mem mem) pc" 
+      by (metis evm_mov)
+
+  hence "disassemble cd \<tturnstile> MS (inv_register_map ps act) (unmap_mem mem) (Suc pc) \<leadsto>\<^sub>m
+    MS (inv_register_map ps act) (unmap_mem mem) pc" by simp
   thus ?case by simp
 next
   case (eva_movk cd pc k mem ps act)
@@ -286,58 +300,58 @@ next
 next
   case (eva_geta cd pc mem r ps t b) 
   hence "disassemble cd ! pc = LOD R5 R5" by simp
-  hence "disassemble cd \<tturnstile> MS (inv_register_map ps (Some r)) (unmap_mem mem) (Suc pc) \<leadsto>\<^sub>m 
-    MS ((inv_register_map ps (Some r))(R5 := unmap_mem mem (inv_register_map ps (Some r) R5))) 
+  hence "disassemble cd \<tturnstile> MS (inv_register_map ps r) (unmap_mem mem) (Suc pc) \<leadsto>\<^sub>m 
+    MS ((inv_register_map ps r)(R5 := unmap_mem mem (inv_register_map ps r R5))) 
       (unmap_mem mem) pc" by (metis evm_lod)
-  with eva_geta(2) show ?case by simp
+  with eva_geta(2, 3) show ?case by simp
 next
   case (eva_get cd pc r mem ps t b act)
   hence "disassemble cd ! pc = LOD R5 (register_map r)" by simp
   hence "disassemble cd \<tturnstile> MS (inv_register_map ps act) (unmap_mem mem) (Suc pc) \<leadsto>\<^sub>m
     MS ((inv_register_map ps act)(R5 := (unmap_mem mem) ((inv_register_map ps act) 
       (register_map r)))) (unmap_mem mem) pc" by (metis evm_lod)
-  with eva_get(2) show ?case by simp
+  with eva_get(2, 3) show ?case by simp
 next
   case (eva_puta cd pc r mem ps act)
   hence "disassemble cd ! pc = STO (register_map r) R5" by simp
   hence "disassemble cd \<tturnstile> MS (inv_register_map ps act) (unmap_mem mem) (Suc pc) \<leadsto>\<^sub>m
     MS (inv_register_map ps act) ((unmap_mem mem)(inv_register_map ps act (register_map r) := 
       inv_register_map ps act R5)) pc" by (metis evm_sto)
-  thus ?case by simp
+  with eva_puta show ?case by simp
 next
   case (eva_putr cd pc r r' mem ps act)
   hence "disassemble cd ! pc = STO (register_map r) (register_map r')" by simp
   hence "disassemble cd \<tturnstile> MS (inv_register_map ps act) (unmap_mem mem) (Suc pc) \<leadsto>\<^sub>m
     MS (inv_register_map ps act) ((unmap_mem mem)(inv_register_map ps act (register_map r) := 
       inv_register_map ps act (register_map r'))) pc" by (metis evm_sto)
-  thus ?case by simp
+  with eva_putr show ?case by simp
 next
   case (eva_putk cd pc r k mem ps act)
   hence "disassemble cd ! pc = STI (register_map r) k" by simp
   hence "disassemble cd \<tturnstile> MS (inv_register_map ps act) (unmap_mem mem) (Suc pc) \<leadsto>\<^sub>m
     MS (inv_register_map ps act) 
       ((unmap_mem mem)(inv_register_map ps act (register_map r) := k)) pc" by (metis evm_sti)
-  thus ?case by (simp add: unmap_upd_k)
+  with eva_putk show ?case by (simp add: unmap_upd_k)
 next
-  case (eva_suba cd pc k ps mem r)
+  case (eva_suba cd pc k ps r mem)
   hence "disassemble cd ! pc = SUB R5 (4 * k)" by simp
-  hence "disassemble cd \<tturnstile> MS (inv_register_map ps (Some r)) (unmap_mem mem) (Suc pc) \<leadsto>\<^sub>m 
-    MS ((inv_register_map ps (Some r))(R5 := inv_register_map ps (Some r) R5 - 4 * k)) 
-      (unmap_mem mem) pc" by (metis evm_sub)
+  hence "disassemble cd \<tturnstile> MS (inv_register_map ps r) (unmap_mem mem) (Suc pc) \<leadsto>\<^sub>m 
+    MS ((inv_register_map ps r)(R5 := inv_register_map ps r R5 - 4 * k)) (unmap_mem mem) pc" 
+      by (metis evm_sub)
   with eva_suba show ?case by simp
 next
-  case (eva_adda cd pc k mem ps r)
+  case (eva_adda cd pc k r mem ps)
   hence "disassemble cd ! pc = ADD R5 (4 * k)" by simp
-  hence "disassemble cd \<tturnstile> MS (inv_register_map ps (Some r)) (unmap_mem mem) (Suc pc) \<leadsto>\<^sub>m 
-    MS ((inv_register_map ps (Some r))(R5 := inv_register_map ps (Some r) R5 + 4 * k)) 
+  hence "disassemble cd \<tturnstile> MS (inv_register_map ps r) (unmap_mem mem) (Suc pc) \<leadsto>\<^sub>m 
+    MS ((inv_register_map ps r)(R5 := inv_register_map ps r R5 + 4 * k)) 
       (unmap_mem mem) pc" by (metis evm_add)
   with eva_adda show ?case by simp
 next
   case (eva_jmp cd pc mem ps)
   hence "disassemble cd ! pc = JMP R5" by simp
-  hence "disassemble cd \<tturnstile> MS (inv_register_map ps None) (unmap_mem mem) (Suc pc) \<leadsto>\<^sub>m 
-    MS ((inv_register_map ps None)(R5 := 0)) (unmap_mem mem) (inv_register_map ps None R5)" 
-      by (metis evm_jmp)
+  hence "disassemble cd \<tturnstile> MS (inv_register_map ps Acc) (unmap_mem mem) (Suc pc) \<leadsto>\<^sub>m 
+    MS ((inv_register_map ps Acc)(R5 := 0)) (unmap_mem mem) (inv_register_map ps Acc R5)" 
+      try by (metis evm_jmp)
   thus ?case by (simp add: inv_reg_map_none)
 qed simp_all
 
@@ -345,29 +359,30 @@ theorem correctm_iter [simp]: "iter (\<tturnstile> cd\<^sub>a \<leadsto>\<^sub>a
     iter (\<tturnstile> disassemble cd\<^sub>a \<leadsto>\<^sub>m) (disassemble_state \<Sigma>\<^sub>a) (disassemble_state \<Sigma>\<^sub>a')"
   by (induction \<Sigma>\<^sub>a \<Sigma>\<^sub>a' rule: iter.induct) (simp, metis correctm iter_append iter_one)
 
-lemma [simp]: "inv_register_map (registers_case 0 0 0 2 0) None = case_reg 0 1 2 11 0" 
+lemma [simp]: "inv_register_map (case_register 0 0 0 2 0) Acc = case_reg 0 1 2 11 0" 
   by (auto split: reg.splits)
 
-lemma [simp]: "inv_register_map (registers_case hp ep (Suc 0) 0 0) None = 
+lemma [simp]: "inv_register_map (case_register hp ep (Suc 0) 0 0) Acc = 
     case_reg (4 * hp) (Suc (4 * ep)) 6 3 0"
   by (auto split: reg.splits)
 
 lemma [dest]: "unmap_mem' x = (r, y) \<Longrightarrow> x = 4 * y + register_offset r"
   by (induction x arbitrary: y rule: unmap_mem'.induct) (simp_all split: prod.splits)
 
-lemma [simp]: "unmap_mem (registers_case (\<lambda>x. (None, 0)) (\<lambda>x. (None, 0)) (\<lambda>x. (None, 0)) 
-  ((\<lambda>x. (None, 0)) (0 := (None, 0), Suc 0 := (Some Env, 0))) undefined) = (\<lambda>x. 0)(7 := 1)"
+lemma [simp]: "unmap_mem (case_register (\<lambda>x. (Acc, 0)) (\<lambda>x. (Acc, 0)) (\<lambda>x. (Acc, 0)) 
+  ((\<lambda>x. (Acc, 0)) (0 := (Acc, 0), Suc 0 := (Env, 0))) undefined) = (\<lambda>x. 0)(7 := 1)"
 proof (rule, unfold unmap_mem_def)
   fix x
   obtain r p where R: "unmap_mem' x = (r, p)" by fastforce
   moreover hence "x = 4 * p + register_offset r" by auto
   ultimately have "pseudoreg_map ((case r of 
-        Stk \<Rightarrow> (\<lambda>x. (None, 0))(0 := (None, 0), Suc 0 := (Some Env, 0)) 
-      | _ \<Rightarrow> (\<lambda>x. (None, 0))) p) = ((\<lambda>x. 0)(3 := 0, 7 := 1)) x" 
-    by (induction r) (simp_all, presburger+)
+        Stk \<Rightarrow> (\<lambda>x. (Acc, 0))(0 := (Acc, 0), Suc 0 := (Env, 0))
+      | Acc \<Rightarrow> undefined 
+      | _ \<Rightarrow> (\<lambda>x. (Acc, 0))) p) = ((\<lambda>x. 0)(3 := 0, 7 := 1)) x" 
+    by (induction r) (simp_all, presburger+, auto)
   with R show "(case unmap_mem' x of (r, p) \<Rightarrow> 
-    pseudoreg_map (registers_case (\<lambda>x. (None, 0)) (\<lambda>x. (None, 0)) (\<lambda>x. (None, 0))
-      ((\<lambda>x. (None, 0))(0 := (None, 0), Suc 0 := (Some Env, 0))) undefined (Some r) p)) =
+    pseudoreg_map (case_register (\<lambda>x. (Acc, 0)) (\<lambda>x. (Acc, 0)) (\<lambda>x. (Acc, 0))
+      ((\<lambda>x. (Acc, 0))(0 := (Acc, 0), Suc 0 := (Env, 0))) undefined r p)) =
         ((\<lambda>x. 0)(7 := 1)) x" by simp
 qed
 
